@prefix concept: <https://data.omgeving.vlaanderen.be/id/concept/lulucf_landgebruikscategorie/>.
@prefix collectie: <https://data.omgeving.vlaanderen.be/id/collection/lulucf_landgebruikscategorie/>.
@prefix access_right: <http://publications.europa.eu/resource/authority/access-right/>.
@prefix adms: <http://www.w3.org/ns/adms#>.
@prefix assettype: <http://purl.org/adms/assettype/>.
@prefix conceptscheme: <https://data.omgeving.vlaanderen.be/id/conceptscheme/lzs/>.
@prefix conceptscheme-alg: <https://data.omgeving.vlaanderen.be/id/conceptscheme/>.
@prefix country: <http://publications.europa.eu/resource/authority/country/>.
@prefix datasets: <https://datasets.omgeving.vlaanderen.be/>.
@prefix datatheme_be: <http://vocab.belgif.be/auth/datatheme/>.
@prefix datatheme_eu: <http://publications.europa.eu/resource/authority/data-theme/>.
@prefix dbo: <http://dbpedia.org/ontology/>.
@prefix dcat: <http://www.w3.org/ns/dcat#>.
@prefix dc: <http://purl.org/dc/elements/1.1/>.
@prefix dct: <http://purl.org/dc/terms/>.
@prefix dr: <https://data.omgeving.vlaanderen.be/id/concept/drager/>.
@prefix eurovoc: <http://eurovoc.europa.eu/>.
@prefix file_type: <http://publications.europa.eu/resource/authority/file-type/>.
@prefix foaf: <http://xmlns.com/foaf/0.1/>.
@prefix formats: <http://www.w3.org/ns/formats/>.
@prefix frequency: <http://publications.europa.eu/resource/authority/frequency/>.
@prefix gemet: <http://www.eionet.europa.eu/gemet/concept/>.
@prefix licence: <http://data.vlaanderen.be/id/licentie/modellicentie-gratis-hergebruik/>.
@prefix cat: <https://data.omgeving.vlaanderen.be/id/concept/lulucf_landgebruikscategorie/>.
@prefix lzs-vocab: <https://data.lzs.omgeving.vlaanderen.be/ns/vocab#>.
@prefix lzs-medium: <https://data.omgeving.vlaanderen.be/id/concept/lzs/medium/>.
@prefix lzs-bandbreedte: <https://data.omgeving.vlaanderen.be/id/concept/lzs/norm_bandbreedte/>.
@prefix lzs-param-norm: <https://data.omgeving.vlaanderen.be/id/concept/lzs/parameter_norm/>.
@prefix lzs-param: <https://data.omgeving.vlaanderen.be/id/concept/lzs/parameter/>.
@prefix lzs-status: <https://data.omgeving.vlaanderen.be/id/concept/lzs/status/>.
@prefix lzs-stalbezetting: <https://data.omgeving.vlaanderen.be/id/concept/lzs/stalbezetting/>.
@prefix lzs-type: <https://data.omgeving.vlaanderen.be/id/concept/lzs/type/>.
@prefix vlarem-klasse: <https://data.omgeving.vlaanderen.be/id/concept/vlarem-klasse/>.
@prefix metadata: <https://data.omgeving.vlaanderen.be/ns/metadata#>.
@prefix omg_catalog_doc: <https://data.omgeving.vlaanderen.be/doc/catalog/>.
@prefix omg_catalog: <https://data.omgeving.vlaanderen.be/id/catalog/>.
@prefix omg_collection: <https://data.omgeving.vlaanderen.be/id/collection/>.
@prefix omg_dataservice: <https://data.omgeving.vlaanderen.be/id/dataservice/>.
@prefix omg_dataset_doc: <https://data.omgeving.vlaanderen.be/doc/dataset/>.
@prefix omg_dataset: <https://data.omgeving.vlaanderen.be/id/dataset/>.
@prefix omg_distribution_doc: <https://data.omgeving.vlaanderen.be/doc/distribution/>.
@prefix omg_distribution: <https://data.omgeving.vlaanderen.be/id/distribution/>.
@prefix omg_graphcollection: <https://data.omgeving.vlaanderen.be/id/graphcollection/>.
@prefix omg_graph: <https://data.omgeving.vlaanderen.be/id/graph/>.
@prefix omg_id: <https://data.omgeving.vlaanderen.be/id/>.
@prefix omg_named_graph: <https://data.omgeving.vlaanderen.be/id/namedgraph/>.
@prefix omg_ontology: <https://data.omgeving.vlaanderen.be/id/ontology/>.
@prefix omg_package: <https://data.omgeving.vlaanderen.be/id/package/>.
@prefix omg_periodoftime: <https://data.omgeving.vlaanderen.be/id/periodoftime/>.
@prefix omg_service: <https://data.omgeving.vlaanderen.be/id/service/>.
@prefix omg_vcard: <https://data.omgeving.vlaanderen.be/id/vcard/>.
@prefix ovo: <http://data.vlaanderen.be/id/organisatie/>.
@prefix owl: <http://www.w3.org/2002/07/owl#>.
@prefix procedure: <https://data.omgeving.vlaanderen.be/id/concept/observatieprocedure/>.
@prefix provenancestatement: <https://data.omgeving.vlaanderen.be/id/provenancestatement/dataset/>.
@prefix quantitykind: <http://qudt.org/vocab/quantitykind/>.
@prefix qudt: <http://qudt.org/schema/qudt/>.
@prefix rdf: <http://www.w3.org/1999/02/22-rdf-syntax-ns#>.
@prefix rdfs: <http://www.w3.org/2000/01/rdf-schema#>.
@prefix repo: <https://repo.omgeving.vlaanderen.be/artifactory/release/>.
@prefix schema: <https://schema.org/>.
@prefix sd: <http://www.w3.org/ns/sparql-service-description#>.
@prefix sh: <http://www.w3.org/ns/shacl#>.
@prefix skos: <http://www.w3.org/2004/02/skos/core#>.
@prefix sosa: <http://www.w3.org/ns/sosa/>.
@prefix spdx: <http://spdx.org/rdf/terms#>.
@prefix ssd: <http://www.w3.org/ns/sparql-service-description#>.
@prefix ssn: <http://www.w3.org/ns/ssn/>.
@prefix ts: <http://www.w3.org/ns/formats/>.
@prefix unit: <http://qudt.org/vocab/unit/>.
@prefix vcard: <http://www.w3.org/2006/vcard/ns#>.
@prefix void: <http://rdfs.org/ns/void#>.
@prefix wise: <http://dd.eionet.europa.eu/vocabulary/wise/ObservedProperty/>.
@prefix xkos: <http://rdf-vocabulary.ddialliance.org/xkos#>.
@prefix xsd: <http://www.w3.org/2001/XMLSchema#>.

<https://data.omgeving.vlaanderen.be/id/concept/lulucf_landgebruikscategorie/100> a skos:Concept;
    skos:definition "All land with woody vegetation that meets the thresholds used to define forest in the national greenhouse gas inventory or that has the potential to meet these thresholds (thresholds; area (ha): 0.5, tree crown cover (%): 20, tree height (m): 5) (Eggleston et al., 2006)."@nl;
    skos:inScheme cat:lulucf_landgebruikscategorie;
    skos:notation "100";
    skos:note "All land with woody vegetation that meets the thresholds used to define forest in the national greenhouse gas inventory or that has the potential to meet these thresholds (thresholds; area (ha): 0.5, tree crown cover (%): 20, tree height (m): 5) (Eggleston et al., 2006)."@nl;
    skos:prefLabel "Forest"@nl;
    skos:topConceptOf cat:lulucf_landgebruikscategorie.
<https://data.omgeving.vlaanderen.be/id/concept/lulucf_landgebruikscategorie/200> a skos:Concept;
    skos:definition "Cultivated land, including rice fields, and agroforestry systems whose vegetation structure falls below the thresholds for the forest category (Eggleston et al., 2006)."@nl;
    skos:inScheme cat:lulucf_landgebruikscategorie;
    skos:notation "200";
    skos:note "Cultivated land, including rice fields, and agroforestry systems whose vegetation structure falls below the thresholds for the forest category (Eggleston et al., 2006)."@nl;
    skos:prefLabel "Cropland"@nl;
    skos:topConceptOf cat:lulucf_landgebruikscategorie.
<https://data.omgeving.vlaanderen.be/id/concept/lulucf_landgebruikscategorie/300> a skos:Concept;
    skos:definition "Pastures and grasslands that are not considered arable land. This category also includes systems with woody vegetation and other vegetation that is not grass, such as herbs and shrubs, that fall below the thresholds for the forest category (Eggleston et al., 2006)."@nl;
    skos:inScheme cat:lulucf_landgebruikscategorie;
    skos:notation "300";
    skos:note "Pastures and grasslands that are not considered arable land. This category also includes systems with woody vegetation and other vegetation that is not grass, such as herbs and shrubs, that fall below the thresholds for the forest category (Eggleston et al., 2006)."@nl;
    skos:prefLabel "Grassland"@nl;
    skos:topConceptOf cat:lulucf_landgebruikscategorie.
<https://data.omgeving.vlaanderen.be/id/concept/lulucf_landgebruikscategorie/400> a skos:Concept;
    skos:definition "Areas with peat extraction and land that is covered or saturated with water throughout all or part of the year (e.g., peatlands) and that does not belong to the categories of forest, cropland, grassland or settlement (Eggleston et al., 2006)."@nl;
    skos:inScheme cat:lulucf_landgebruikscategorie;
    skos:notation "400";
    skos:note "Areas with peat extraction and land that is covered or saturated with water throughout all or part of the year (e.g., peatlands) and that does not belong to the categories of forest, cropland, grassland or settlement (Eggleston et al., 2006)."@nl;
    skos:prefLabel "Wetland"@nl;
    skos:topConceptOf cat:lulucf_landgebruikscategorie.
<https://data.omgeving.vlaanderen.be/id/concept/lulucf_landgebruikscategorie/500> a skos:Concept;
    skos:definition "All developed land, including transport infrastructure and residential areas of any size, unless they already fall under other categories such as forest, cropland, grassland or wetland (Eggleston et al., 2006)."@nl;
    skos:inScheme cat:lulucf_landgebruikscategorie;
    skos:narrower <https://data.omgeving.vlaanderen.be/id/concept/lulucf_landgebruikscategorie/501>, <https://data.omgeving.vlaanderen.be/id/concept/lulucf_landgebruikscategorie/502>;
    skos:narrowerTransitive <https://data.omgeving.vlaanderen.be/id/concept/lulucf_landgebruikscategorie/501>, <https://data.omgeving.vlaanderen.be/id/concept/lulucf_landgebruikscategorie/502>;
    skos:notation "500";
    skos:note "All developed land, including transport infrastructure and residential areas of any size, unless they already fall under other categories such as forest, cropland, grassland or wetland (Eggleston et al., 2006)."@nl;
    skos:prefLabel "Settlement"@nl;
    skos:semanticRelation <https://data.omgeving.vlaanderen.be/id/concept/lulucf_landgebruikscategorie/501>, <https://data.omgeving.vlaanderen.be/id/concept/lulucf_landgebruikscategorie/502>;
    skos:topConceptOf cat:lulucf_landgebruikscategorie.
<https://data.omgeving.vlaanderen.be/id/concept/lulucf_landgebruikscategorie/501> a skos:Concept;
    skos:broader <https://data.omgeving.vlaanderen.be/id/concept/lulucf_landgebruikscategorie/500>;
    skos:broaderTransitive <https://data.omgeving.vlaanderen.be/id/concept/lulucf_landgebruikscategorie/500>;
    skos:definition "All sealed developed land of the category settlement."@nl;
    skos:inScheme cat:lulucf_landgebruikscategorie;
    skos:notation "501";
    skos:note "All sealed developed land of the category settlement."@nl;
    skos:prefLabel "Sealed settlement"@nl;
    skos:semanticRelation <https://data.omgeving.vlaanderen.be/id/concept/lulucf_landgebruikscategorie/500>.
<https://data.omgeving.vlaanderen.be/id/concept/lulucf_landgebruikscategorie/502> a skos:Concept;
    skos:broader <https://data.omgeving.vlaanderen.be/id/concept/lulucf_landgebruikscategorie/500>;
    skos:broaderTransitive <https://data.omgeving.vlaanderen.be/id/concept/lulucf_landgebruikscategorie/500>;
    skos:definition "All unsealed developed land of the category settlement."@nl;
    skos:inScheme cat:lulucf_landgebruikscategorie;
    skos:notation "502";
    skos:note "All unsealed developed land of the category settlement."@nl;
    skos:prefLabel "Unsealed settlement"@nl;
    skos:semanticRelation <https://data.omgeving.vlaanderen.be/id/concept/lulucf_landgebruikscategorie/500>.
cat:lulucf_landgebruikscategorie a skos:ConceptScheme;
    skos:definition "This code list contains an overview of the Flemish land use categories used in the context of the European LULUCF Regulation regarding the reporting of greenhouse gas storage and emissions related to land use changes. "@nl;
    skos:hasTopConcept <https://data.omgeving.vlaanderen.be/id/concept/lulucf_landgebruikscategorie/100>, <https://data.omgeving.vlaanderen.be/id/concept/lulucf_landgebruikscategorie/200>, <https://data.omgeving.vlaanderen.be/id/concept/lulucf_landgebruikscategorie/300>, <https://data.omgeving.vlaanderen.be/id/concept/lulucf_landgebruikscategorie/400>, <https://data.omgeving.vlaanderen.be/id/concept/lulucf_landgebruikscategorie/500>;
    skos:note "This code list contains an overview of the Flemish land use categories used in the context of the European LULUCF Regulation regarding the reporting of greenhouse gas storage and emissions related to land use changes. "@nl;
    skos:prefLabel "LULUCF land use categories"@nl.
